more

thys/Substitution/Expression_Like_Birecursor.thy
@@ -7,11 +7,11 @@ locale Bimodel = Nominal Pperm "PVrs :: 'p \<Rightarrow> 'a :: var set" + Expres
   fixes  is_base :: "('a::var, 'a, 'e, 'e) G \<Rightarrow> bool"
   and Ector_base :: "('a::var, 'a, 'e, 'e) G \<Rightarrow> 'p \<Rightarrow> 'e"
   and Ector_step :: "('a::var, 'a, 'p \<Rightarrow> 'e, 'p \<Rightarrow> 'e) G \<Rightarrow> 'p \<Rightarrow> 'e"
-  assumes "\<exists>P. P is_base Ector_base Ector_step"
+  assumes TODO: "\<exists>P. P is_base Ector_base Ector_step"
 
 locale Birecursor = Bimodel Pperm "PVrs :: 'p \<Rightarrow> 'a set" Eperm "EVrs :: 'e \<Rightarrow> 'a :: var set" Ector is_base Ector_base Ector_step
   for Pperm PVrs Eperm EVrs Ector is_base Ector_base Ector_step +
-  assumes rec: "\<exists>!rec.
+  assumes rec: "\<exists>rec.
       ((\<forall>u p. is_base u \<longrightarrow> GVrs2 u \<inter> PVrs p = {} \<longrightarrow> rec (Ector u) p = Ector_base u p) \<and>
        (\<forall>u p. \<not> is_base u \<longrightarrow> GVrs2 u \<inter> PVrs p = {} \<longrightarrow> rec (Ector u) p = Ector_step (Gmap rec rec u) p) \<and>
        (\<forall>e p \<sigma>. bij \<sigma> \<longrightarrow> |supp \<sigma>| <o |UNIV :: 'a set| \<longrightarrow> rec (Eperm \<sigma> e) p = Eperm \<sigma> (rec e (Pperm (inv \<sigma>) p))) \<and>
@@ -19,25 +19,25 @@ locale Birecursor = Bimodel Pperm "PVrs :: 'p \<Rightarrow> 'a set" Eperm "EVrs 
 begin
 
 definition rec where
-  "rec = (THE rec. ((\<forall>u p. is_base u \<longrightarrow> GVrs2 u \<inter> PVrs p = {} \<longrightarrow> rec (Ector u) p = Ector_base u p) \<and>
+  "rec = (SOME rec. ((\<forall>u p. is_base u \<longrightarrow> GVrs2 u \<inter> PVrs p = {} \<longrightarrow> rec (Ector u) p = Ector_base u p) \<and>
        (\<forall>u p. \<not> is_base u \<longrightarrow> GVrs2 u \<inter> PVrs p = {} \<longrightarrow> rec (Ector u) p = Ector_step (Gmap rec rec u) p) \<and>
        (\<forall>e p \<sigma>. bij \<sigma> \<longrightarrow> |supp \<sigma>| <o |UNIV :: 'a set| \<longrightarrow> rec (Eperm \<sigma> e) p = Eperm \<sigma> (rec e (Pperm (inv \<sigma>) p))) \<and>
        (\<forall>e p. EVrs (rec e p) \<subseteq> PVrs p \<union> EVrs e)))"
 
 lemma rec_base: "is_base u \<Longrightarrow> GVrs2 u \<inter> PVrs p = {} \<Longrightarrow> rec (Ector u) p = Ector_base u p"
-  using theI'[OF rec, THEN conjunct1] unfolding rec_def
+  using someI_ex[OF rec, THEN conjunct1] unfolding rec_def
   by blast
 
 lemma rec_Ector: "\<not> is_base u \<Longrightarrow> GVrs2 u \<inter> PVrs p = {} \<Longrightarrow> rec (Ector u) p = Ector_step (Gmap rec rec u) p"
-  using theI'[OF rec, THEN conjunct2, THEN conjunct1] unfolding rec_def
+  using someI_ex[OF rec, THEN conjunct2, THEN conjunct1] unfolding rec_def
   by blast
 
 lemma rec_EPerm: "bij \<sigma> \<Longrightarrow> |supp \<sigma>| <o |UNIV :: 'a set| \<Longrightarrow> rec (Eperm \<sigma> e) p = Eperm \<sigma> (rec e (Pperm (inv \<sigma>) p))"
-  using theI'[OF rec, THEN conjunct2, THEN conjunct2, THEN conjunct1] unfolding rec_def
+  using someI_ex[OF rec, THEN conjunct2, THEN conjunct2, THEN conjunct1] unfolding rec_def
   by blast
 
 lemma rec_EVrs: "EVrs (rec e p) \<subseteq> PVrs p \<union> EVrs e"
-  using theI'[OF rec, THEN conjunct2, THEN conjunct2, THEN conjunct2] unfolding rec_def
+  using someI_ex[OF rec, THEN conjunct2, THEN conjunct2, THEN conjunct2] unfolding rec_def
   by blast
 
 end
@@ -78,7 +78,7 @@ lemma permute_\<rho>':
    apply (auto simp: IImsupp'_def IImsupp_def SSupp_def imsupp_def supp_def)
   done
 
-sublocale Esub: Bimodel where
+sublocale Esub: Birecursor where
   Pperm = "\<lambda>\<sigma> (\<delta>, \<rho>, \<rho>'). (\<sigma> o \<delta> o inv \<sigma>, Eperm \<sigma> o \<rho> o inv \<sigma>, Eperm \<sigma> o \<rho>' o inv \<sigma>)" and
   PVrs = "\<lambda>(\<delta>, \<rho>, \<rho>'). imsupp \<delta> \<union> IImsupp' (Ector \<circ> \<eta>) EVrs \<rho> \<union> IImsupp' (Ector \<circ> \<eta>') EVrs \<rho>'" and
   Eperm = Eperm and
@@ -86,7 +86,7 @@ sublocale Esub: Bimodel where
   Ector = Ector and
   is_base = "\<lambda>u. \<exists>a. u = \<eta> a \<or> u = \<eta>' a" and
   Ector_base = "\<lambda>u (\<delta>, \<rho>, \<rho>'). if (\<exists>a. u = \<eta> a) then \<rho> (SOME a. u = \<eta> a) else \<rho>' (SOME a. u = \<eta>' a)" and
-  Ector_step = "\<lambda>u (\<delta>, \<rho>, \<rho>'). Ector (Gmap (\<lambda>rec. rec (\<delta>, \<rho>, \<rho>')) (\<lambda>rec. rec (\<delta>, \<rho>, \<rho>')) u)"
+  Ector_step = "\<lambda>u (\<delta>, \<rho>, \<rho>'). Ector (Gsub \<delta> id (Gmap (\<lambda>rec. rec (\<delta>, \<rho>, \<rho>')) (\<lambda>rec. rec (\<delta>, \<rho>, \<rho>')) u))"
   apply standard
   subgoal for \<sigma> \<tau>
     by (auto simp: fun_eq_iff o_inv_distrib Eperm_comp[THEN fun_cong, simplified])
@@ -99,20 +99,28 @@ sublocale Esub: Bimodel where
     done
   subgoal
     sorry
+  subgoal
+    sorry
   done
 
-sublocale rec: Birecursor
+definition "Esub \<delta> \<rho> \<rho>' e = Esub.rec e (\<delta>, \<rho>, \<rho>')"
+
+interpretation Substitution Eperm EVrs Ector Esub
   apply standard
-
-end
-
-context Birecursor begin
-
-term Esub.rec
-
-interpretation Substitution undefined
-  apply standard
-  sorry
+      apply (unfold Esub_def)
+      apply (subst Esub.rec_base; auto simp add: eta_inject)
+      apply (subst Esub.rec_base; auto simp add: eta_distinct' eta'_inject)
+    apply (subst Esub.rec_Ector; auto simp add: G.Map_comp[THEN fun_cong, simplified] comp_def[of _ Esub.rec])
+   apply (rule order_trans[OF Esub.rec_EVrs]; simp)
+  apply (subst Esub.rec_EPerm; simp)
+  apply (rule arg_cong[where f = "\<lambda>p. Eperm _ (Esub.rec _ p)"])
+  apply (auto simp: fun_eq_iff)
+  apply (metis Int_Un_empty Int_emptyD bij_inv_rev imsupp_idle2 not_in_imsupp_same)
+  apply (metis (mono_tags, lifting) Int_Un_empty Int_Un_emptyI1 bij_betw_inv_into imsupp_inv inv_simp1
+      permute_\<rho> supp_inv_bound)
+  apply (smt (verit, best) Int_Un_empty Un_commute bij_betw_inv_into imsupp_inv inv_simp1 permute_\<rho>'
+      supp_inv_bound)
+  done
 
 end
 
